Completed some lemmas for proposition 1. Updated obs to be a finite set.

Hyperproperties.v
@@ -1,3 +1,4 @@
+From Coq Require Import Arith.
 From Coq Require Import Lists.List. Import ListNotations.
 From Coq Require Import Lists.Streams.
 From Coq Require Import Sets.Ensembles.
@@ -6,11 +7,16 @@ From Coq Require Import Sets.Finite_sets.
 From Coq Require Import Sets.Constructive_sets.
 From Coq Require Import Logic.Classical_Prop.
 From Coq Require Import Logic.Classical_Pred_Type.
-
+From Coq Require Import Lists.ListSet.
+From Coq Require Import Structures.Equalities.
+Scheme Equality for list.
 
 Module Type StateTypeMod.
   Parameter StateType: Type.
   (* TODO(ptcrews): We probably need equality axioms here *)
+  Parameter eq_dec: forall x y: StateType, {x = y} + {x <> y}.
+  Parameter eqb: StateType -> StateType -> bool.
+  Parameter eqb_eq: forall x y: StateType, eqb x y = true <-> x = y.
 End StateTypeMod.
 
 Module Hyperproperty (SM: (StateTypeMod)).
@@ -40,7 +46,7 @@ Lemma Rewrite_Included_satisfies_property : forall (s : system) (P : property),
 Proof. reflexivity. Qed.
 
 Lemma Rewrite_In_satisfies_hyperproperty : forall (s : system) (Hp : hyperproperty),
-  In system Hp s = satisfies_hyperproperty s Hp.
+  Ensembles.In system Hp s = satisfies_hyperproperty s Hp.
 Proof. reflexivity. Qed.
 
 Definition lift (P : property) : hyperproperty := Power_set trace P.
@@ -63,12 +69,12 @@ Inductive prefix : trace -> subtrace -> Prop :=
 
 Definition prefix_set
   (traces : Ensemble trace)
-  (prefixes : Ensemble subtrace) :=
+  (prefixes : set subtrace) :=
   forall (p : subtrace),
-  In (subtrace) prefixes p -> exists (t: trace), In (trace) traces t /\ prefix t p.
+  set_In p prefixes -> exists (t: trace), In (trace) traces t /\ prefix t p.
 
 (* Definition Obs :=  Full_set (Ensemble subtrace). *)
-Definition Obs := Ensemble subtrace.
+Definition Obs := set subtrace.
 
 Definition safety_property (p: property) :=
   forall (t : trace),
@@ -86,30 +92,66 @@ Definition SP := { p:property | safety_property p}.
 (* The set of all Safety Hyperproperties *)
 Definition SHP := { h:hyperproperty | safety_hyperproperty h}.
 
-
-
-
-
 Lemma not_included_gives_exists : forall (p : property) (s : system),
   ~ Included trace s p -> exists t : trace, ~ In trace p t /\ In trace s t.
 Proof. intros p s H. unfold Included in H. apply not_all_ex_not in H. destruct H.
 exists x.  apply imply_to_and   in H. destruct H. split.
 + apply H0.
 + apply H.
-Qed. 
+Qed.
 
-Lemma inhabited_gives_exists: forall (U: Type) (A:Ensemble U),
-  Inhabited U A -> exists x : U, In U A x.
-Proof. Admitted.
+Fixpoint max_prefix (prefix: set subtrace) : option subtrace :=
+  match prefix with
+  | nil => None
+  | p :: prefix =>
+      match max_prefix prefix with
+      | None => Some p
+      | Some p' => if (length p) <=? (length p') then Some p' else Some p
+      end
+  end.
 
-Lemma prefix_set_Singleton : forall (t : trace) (prefixes : Ensemble subtrace),
-  Inhabited subtrace prefixes /\ prefix_set (Singleton trace t) prefixes ->
-  exists p : subtrace, In subtrace prefixes p /\
+Lemma non_empty_gives_max_prefix: forall (prefixes : set subtrace),
+  prefixes <> (empty_set subtrace) ->
+  exists p: subtrace, max_prefix prefixes = Some p.
+Proof.
+  intros. destruct prefixes.
+  - contradiction.
+  - destruct (max_prefix (s::prefixes)) eqn:H'.
+    + exists s0. reflexivity.
+    + inversion H'. destruct (max_prefix prefixes).
+      ++ destruct (length s <=? length s0); inversion H1.
+      ++ inversion H1.
+Qed.
+
+Lemma max_prefix_gives_element: forall (prefixes: set subtrace) (p: subtrace),
+  max_prefix prefixes = Some p -> set_In p prefixes.
+Proof.
+  intros. induction prefixes.
+  - inversion H.
+  - destruct (list_eq_dec _ eqb) with p a as [H1|H2]; try apply eqb_eq.
+    + rewrite H1 in *. simpl. left. reflexivity.
+    + simpl. right. apply IHprefixes. simpl in H.
+      assert (Hneq: Some a <> Some p). { congruence. }
+      destruct (max_prefix prefixes).
+      ++ destruct (length a <=? length s).
+         +++ apply H.
+         +++ contradiction.
+      ++ contradiction.
+Qed.
+
+Lemma prefix_set_Singleton : forall (t : trace) (prefixes : set subtrace),
+  prefixes <> (empty_set subtrace) /\ prefix_set (Singleton trace t) prefixes ->
+  exists p : subtrace, set_In p prefixes /\
   (forall t' : trace, prefix t' p -> prefix_set (Singleton trace t') prefixes).
-intros t prefixes.
-Proof. Admitted.
-
-
+Proof.
+intros t prefixes H. destruct H as [H H']. unfold prefix_set in H'.
+apply non_empty_gives_max_prefix in H. destruct H as [p H1]. exists p.
+split.
+- apply max_prefix_gives_element. apply H1.
+- intros. unfold prefix_set. intros. exists t'. split.
+  + apply In_singleton.
+  + admit.
+Admitted.
 
 Theorem lifting_preserves_safety:
   forall (p : property), safety_property p <-> safety_hyperproperty [[p]].
@@ -122,15 +164,16 @@ Proof.
     apply not_included_gives_exists in H'. destruct H' as [t H''].
     destruct H'' as [Hp Hs].
     specialize (H t). apply H in Hp. destruct Hp as [m Hp'].
-    exists (Singleton subtrace m). intros s'. split.
-    + unfold prefix_set. intros p' H0. apply Singleton_inv in H0.
-      rewrite H0 in *. exists t. split.
+    exists [m]. intros s'. split.
+    + unfold prefix_set. intros p' H0. inversion H0.
+      rewrite H1 in *. exists t. split.
       ++ apply Hs.
-      ++ destruct (Hp' t). apply H1.
+      ++ destruct (Hp' t). apply H2.
+      ++ inversion H1.
     + intros Hpset. rewrite Rewrite_In_satisfies_hyperproperty.
       rewrite <- lifting_preserves_satisfiability.
       unfold satisfies_property. unfold prefix_set in Hpset. destruct (Hpset m).
-      ++ apply In_singleton.
+      ++ simpl. left. reflexivity.
       ++ intros contra. unfold Included in contra. specialize (contra x).
          destruct H0 as [H0 H0'].
          apply contra in H0. specialize (Hp' x). destruct Hp' as [Hp' Hp''].
@@ -144,14 +187,13 @@ Proof.
       apply H' in contra.
       ++ apply contra.
       ++ apply In_singleton.
-    + assert (Hinhabited: Inhabited subtrace x
+    + assert (Hinhabited: x <> empty_set subtrace
                           /\ prefix_set (Singleton trace t) x). {
         destruct (H0 (Singleton trace t)) as [H0' H0''].
         split.
         - apply H0'' in H0'. apply NNPP. unfold not. intros.
           destruct (H0 p) as [H2 H2']. destruct H2'.
-          + unfold prefix_set. intros. apply Inhabited_intro in H3.
-            apply H1 in H3. contradiction.
+          + unfold prefix_set. intros. apply NNPP in H1. rewrite H1 in H3. inversion H3.
           + unfold lift. unfold In. apply Definition_of_Power_set.
             unfold Included. intros. apply H3.
         - apply H0'.
